AsyncTest module WIP

theories/Trace.v
@@ -1,6 +1,16 @@
 From JSON Require Export
      JSON.
 
+Definition clientT := nat.
+Variant connT :=
+  Conn__Server
+| Conn__Client : clientT -> connT.
+
+Record packetT :=
+  Packet { packet__src     : connT;
+           packet__dst     : connT;
+           packet__payload : json }.
+
 Definition labelT := nat.
 
-Definition traceT := list (labelT * json).
+Definition traceT := list (labelT * packetT).
