theories/AsyncTest.v
@@ -1,0 +1,76 @@
+From QuickChick Require Export
+     QuickChick.
+From ITree Require Export
+     Exception
+     ITree.
+From SimpleIO Require Export
+     SimpleIO.
+From AsyncTest Require Export
+     Instances.
+
+Variant clientE {gen_state} : Type -> Type :=
+  Client__Recv :             clientE (option packetT)
+| Client__Send : gen_state -> clientE (option packetT).
+
+Module Type AsyncTestSIG.
+
+Parameter gen_state     : Type.
+Parameter otherE        : Type -> Type.
+Parameter other_handler : otherE ~> IO.
+Arguments other_handler {_}.
+
+Notation failureE       := (exceptE string).
+Notation tE             := (failureE +' @clientE gen_state +' otherE).
+
+Parameter conn_state    : Type.
+Parameter init_state    : conn_state.
+Parameter recv_response : Monads.stateT conn_state IO (option packetT).
+Parameter send_request  : connT -> json -> Monads.stateT conn_state IO unit.
+Parameter cleanup       : conn_state -> IO unit.
+
+Parameter gen_request   : gen_state -> traceT -> IO (clientT * jexp).
+
+Parameter tester_state  : Type.
+Parameter tester_init   : IO tester_state.
+Parameter tester        : tester_state -> itree tE void.
+
+End AsyncTestSIG.
+
+Module AsyncTest (SIG : AsyncTestSIG).
+Include SIG.
+
+Notation scriptT := (list (clientT * jexp)).
+
+Definition shrink_execute' (exec : scriptT -> IO (bool * traceT))
+           (init : scriptT) : IO (option scriptT) :=
+  prerr_endline "===== initial script =====";;
+  prerr_endline (to_string init);;
+  IO.fix_io
+    (fun shrink_rec ss =>
+       match ss with
+       | [] => prerr_endline "<<<<< shrink exhausted >>>>";; ret None
+       | sc :: ss' =>
+         prerr_endline "<<<<< current script >>>>>>";;
+         prerr_endline (to_string sc);;
+         '(b, tr) <- exec sc;;
+         if b : bool
+         then prerr_endline "===== accepting trace =====";;
+              prerr_endline (to_string tr);;
+              shrink_rec ss'
+         else prerr_endline "===== rejecting trace =====";;
+              prerr_endline (to_string tr);;
+              prerr_endline "<<<<< shrink ended >>>>>>>>";;
+              ret (Some sc)
+       end) (repeat_list 20 $ shrink init).
+
+Definition shrink_execute (first_exec : IO (bool * (scriptT * traceT)))
+           (then_exec : scriptT -> IO (bool * traceT)) : IO bool :=
+  '(b, (sc, tr)) <- first_exec;;
+  if b : bool
+  then ret true
+  else prerr_endline "<<<<< rejecting trace >>>>>";;
+       prerr_endline (to_string tr);;
+       IO.while_loop (shrink_execute' then_exec) sc;;
+       ret false.
+
+End AsyncTest.
