theories/Instances.v
@@ -1,0 +1,66 @@
+From QuickChick Require Export
+     QuickChick.
+From JSON Require Export
+     Instances.
+From AsyncTest Require Export
+     Jexp.
+
+Definition shrinkValue {K V} (shr : V -> list V)
+  : list (K * V) -> list (list (K * V)) :=
+  shrinkListAux (fun kv => let (k, v) := kv : K * V in
+                        map (pair k) $ shr v).
+
+Instance Shrink__json : Shrink json :=
+  {| shrink :=
+       fix shrink_json (j : json) : list json :=
+         match j with
+         | JSON__Number n => map JSON__Number $ shrink n
+         (* | JSON__Array  l => map JSON__Array  $ shrinkListAux shrink_json l *)
+         (* | JSON__Object l => map JSON__Object $ shrinkValue   shrink_json l *)
+         | _            => []
+         end |}.
+
+Instance Shrink__jexp : Shrink jexp :=
+  {| shrink :=
+       fix shrink_jexp (e : jexp) : list jexp :=
+         match e with
+         | Jexp__Const  j => map Jexp__Const  $ shrink j
+         (* | Jexp__Array  l => map Jexp__Array  $ shrinkListAux shrink_jexp l *)
+         (* | Jexp__Object l => map Jexp__Object $ shrinkValue   shrink_jexp l *)
+         | _ => []
+         end |}.
+
+Instance Serialize__jpath : Serialize jpath :=
+  let fix jpath_to_list (p : jpath) : list sexp :=
+      match p with
+      | Jpath__This       => []
+      | Jpath__Array  n p => to_sexp n::jpath_to_list p
+      | Jpath__Object s p => Atom s   ::jpath_to_list p
+      end in
+  List ∘ jpath_to_list.
+
+Local Open Scope sexp_scope.
+
+Instance Serialize__connT : Serialize connT :=
+  fun c =>
+    match c with
+    | Conn__Client c => [Atom "Client"; to_sexp c]
+    | Conn__Server   => [Atom "Server"]
+    end.
+
+Instance Serialize__packetT : Serialize packetT :=
+  fun pkt =>
+    let 'Packet s d p := pkt in
+    [[Atom "Src"; to_sexp s];
+     [Atom "Dst"; to_sexp d];
+     [Atom "Msg"; to_sexp p]].
+
+Instance Serialize__jexp : Serialize jexp :=
+  fix jexp_to_sexp (e : jexp) : sexp :=
+    match e with
+    | Jexp__Const  j => to_sexp j
+    | Jexp__Array  l => List $ map jexp_to_sexp l
+    | Jexp__Object l => List $ map (fun se => let (s, e) := se : string * jexp in
+                                        [Atom s; jexp_to_sexp e]) l
+    | Jexp__Ref  l p => [[Atom "label"; to_sexp l]; [Atom "path"; to_sexp p]]
+    end.
